@prefix bot: <https://w3id.org/bot#> .
@prefix ioe: <http://w3id.org/semioe#> .
@prefix org: <http://www.w3.org/ns/org#> .
@prefix owl: <http://www.w3.org/2002/07/owl#> .
@prefix rdf: <http://www.w3.org/1999/02/22-rdf-syntax-ns#> .
@prefix ssn: <http://www.w3.org/ns/ssn/> .
@prefix xml: <http://www.w3.org/XML/1998/namespace> .
@prefix xsd: <http://www.w3.org/2001/XMLSchema#> .
@prefix foaf: <http://xmlns.com/foaf/0.1/> .
@prefix rdfs: <http://www.w3.org/2000/01/rdf-schema#> .
@prefix vann: <http://purl.org/vocab/vann/> .
@prefix dcterms: <http://purl.org/dc/terms/> .

<http://w3id.org/semioe#> rdf:type owl:Ontology ;
                           owl:imports org: ;
                           <http://purl.org/dc/elements/1.1/created> "2023/12/20 18:44:00" ;
                           <http://purl.org/dc/elements/1.1/title> "SemIoE" ;
                           dcterms:creator [ rdf:type foaf:Agent ;
                                             foaf:homepage <https://orcid.org/0000-0001-5966-6921> ;
                                             foaf:name "Emanuele Storti"
                                           ] ,
                                           [ rdf:type foaf:Agent ;
                                             foaf:homepage <https://orcid.org/0000-0003-2120-2341> ;
                                             foaf:name "Antonino Nocera"
                                           ] ,
                                           [ rdf:type foaf:Agent ;
                                             foaf:homepage <https://orcid.org/0000-0002-3371-307X> ;
                                             foaf:name "Marco Arazzi"
                                           ] ;
                           dcterms:license <https://creativecommons.org/licenses/by/4.0> ;
                           vann:preferredNamespacePrefix "ioe" ;
                           vann:preferredNamespaceUri <https://w3id.org/semioe#> ;
                           rdfs:comment "The SemIoE ontology is aimed to represent resources and their relations in a Internet-of-Everything network." ;
                           rdfs:label "SemIoE" ;
                           owl:versionInfo "0.9" .

#################################################################
#    Annotation properties
#################################################################

###  http://purl.org/dc/elements/1.1/created
<http://purl.org/dc/elements/1.1/created> rdf:type owl:AnnotationProperty .


###  http://purl.org/dc/elements/1.1/title
<http://purl.org/dc/elements/1.1/title> rdf:type owl:AnnotationProperty .


###  http://purl.org/dc/terms/creator
dcterms:creator rdf:type owl:AnnotationProperty .


###  http://purl.org/vocab/vann/preferredNamespacePrefix
vann:preferredNamespacePrefix rdf:type owl:AnnotationProperty ;
                              rdfs:subPropertyOf vann:preferredNamespacePrefix .


###  http://purl.org/vocab/vann/preferredNamespaceUri
vann:preferredNamespaceUri rdf:type owl:AnnotationProperty .


###  http://xmlns.com/foaf/0.1/maker
foaf:maker rdf:type owl:AnnotationProperty .


#################################################################
#    Object Properties
#################################################################

###  http://w3id.org/semioe#engagedIn
ioe:engagedIn rdf:type owl:ObjectProperty ;
              rdfs:domain ioe:Agent ;
              rdfs:range ioe:Activity ;
              rdfs:comment "Relates an ioe:Agent to the ioe:Activity which she/he is engaged with." ;
              rdfs:label "engagedIn" .


###  http://w3id.org/semioe#forRole
ioe:forRole rdf:type owl:ObjectProperty ;
            rdfs:domain ioe:Right ;
            rdfs:range ioe:CurrentRole .


###  http://w3id.org/semioe#forWorkflowElement
ioe:forWorkflowElement rdf:type owl:ObjectProperty ;
                       rdfs:domain ioe:AgentRelation ;
                       rdfs:range ioe:WorkflowElement ;
                       rdfs:comment "Relates an ioe:ActorRelation with the ioe:WorkflowElement for which the relation is established." ;
                       rdfs:label "forWorkflowElement" .


###  http://w3id.org/semioe#fromAgent
ioe:fromAgent rdf:type owl:ObjectProperty ;
              rdfs:domain ioe:AgentRelation ;
              rdfs:range ioe:Agent ;
              rdfs:comment "Relates an ioe:ActorRelation to the ioe:Agent initiating the relation." ;
              rdfs:label "fromAgent" .


###  http://w3id.org/semioe#hasType
ioe:hasType rdf:type owl:ObjectProperty ;
            rdfs:domain ioe:Right ;
            rdfs:range ioe:RightType ;
            rdfs:comment "Specifies the type of a ioe:Right" ;
            rdfs:label "hasType" .


###  http://w3id.org/semioe#inProcess
ioe:inProcess rdf:type owl:ObjectProperty ;
              rdfs:domain ioe:Activity ;
              rdfs:range ioe:Process ;
              rdfs:comment "Relates an ioe:Activity to the ioe:Process to which it belongs" ;
              rdfs:label "inProcess" .


###  http://w3id.org/semioe#includedIn
ioe:includedIn rdf:type owl:ObjectProperty ,
                        owl:FunctionalProperty ;
               rdfs:domain ioe:System ;
               rdfs:range ioe:SmartObject ;
              rdfs:comment "Relates an ioe:System to the ioe:SmartObject which includes it" ;
              rdfs:label "includedIn" .



###  http://w3id.org/semioe#locatedIn
ioe:locatedIn rdf:type owl:ObjectProperty ,
                       owl:FunctionalProperty ;
              rdfs:domain ioe:Agent ;
              rdfs:range ioe:Site ;
              rdfs:comment "Relates an ioe:Agent to the ioe:Site in which she/he is located." ;
              rdfs:label "locatedIn" .


###  http://w3id.org/semioe#onEnvironment
ioe:onEnvironment rdf:type owl:ObjectProperty ;
                  rdfs:domain ioe:RightOnEnvironment ;
                  rdfs:range ioe:Site ;
                  rdfs:comment "Specifies the ioe:Site on which the ioe:RightOnEnvironment applies." ;
                  rdfs:label "onEnvironment" .


###  http://w3id.org/semioe#onSmartObject
ioe:onSmartObject rdf:type owl:ObjectProperty ;
                  rdfs:domain ioe:RightOnSmartObject ;
                  rdfs:range ioe:SmartObject ;
                  rdfs:comment "Specifies the ioe:SmartObject on which the ioe:RightOnSmartObject applies." ;
                  rdfs:label "onSmartObject" .


###  http://w3id.org/semioe#onSystem
ioe:onSystem rdf:type owl:ObjectProperty ;
             rdfs:domain ioe:RightOnSystem ;
             rdfs:range ssn:System ;
             rdfs:comment "Specifies the ssn:System on which the ioe:RightOnSystem applies." ;
             rdfs:label "onSystem" .


###  http://w3id.org/semioe#toAgent
ioe:toAgent rdf:type owl:ObjectProperty ;
            rdfs:domain ioe:AgentRelation ;
            rdfs:range ioe:Agent ;
            rdfs:comment "Relates an ioe:ActorRelation to the ioe:Agent that is the object of the relation." ;
            rdfs:label "toAgent" .


#################################################################
#    Data properties
#################################################################

###  http://w3id.org/semioe#endTime
ioe:endTime rdf:type owl:DatatypeProperty ;
            rdfs:domain ioe:CurrentRole ;
            rdfs:range xsd:dateTime ;
            rdfs:comment "The dateTime representing the end of the relation" ;
            rdfs:label "endTime" .


###  http://w3id.org/semioe#isTransferrable
ioe:isTransferrable rdf:type owl:DatatypeProperty ;
                    rdfs:domain ioe:CurrentRole ;
                    rdfs:range xsd:boolean ;
                    rdfs:comment "Specifies whether an ioe:CurrentRole can be transferred from an ioe:Agent to another" ;
                    rdfs:label "isTransferrable" .


###  http://w3id.org/semioe#startTime
ioe:startTime rdf:type owl:DatatypeProperty ;
              rdfs:domain ioe:CurrentRole ;
              rdfs:range xsd:dateTime ;
              rdfs:comment "The dateTime representing the start of the relation" ;
              rdfs:label "startTime" .


#################################################################
#    Classes
#################################################################

###  http://w3id.org/semioe#Activity
ioe:Activity rdf:type owl:Class ;
             rdfs:subClassOf ioe:WorkflowElement ;
             rdfs:comment "An activity in a ioe:Process of the organization." ;
             rdfs:label "Activity" .


###  http://w3id.org/semioe#Agent
ioe:Agent rdf:type owl:Class ;
          owl:equivalentClass [ rdf:type owl:Restriction ;
                                owl:onProperty ioe:locatedIn ;
                                owl:qualifiedCardinality "1"^^xsd:nonNegativeInteger ;
                                owl:onClass ioe:Site
                              ] ;
          rdfs:comment "An agent in the IoE network. The class is a generalization of foaf:Agent and ioe:SmartObject." ;
          rdfs:label "Agent" .


###  http://w3id.org/semioe#AgentRelation
ioe:AgentRelation rdf:type owl:Class ;
                  rdfs:subClassOf [ rdf:type owl:Restriction ;
                                    owl:onProperty ioe:forWorkflowElement ;
                                    owl:someValuesFrom ioe:Activity
                                  ] ,
                                  [ rdf:type owl:Restriction ;
                                    owl:onProperty ioe:fromAgent ;
                                    owl:someValuesFrom ioe:Agent
                                  ] ,
                                  [ rdf:type owl:Restriction ;
                                    owl:onProperty ioe:toAgent ;
                                    owl:someValuesFrom ioe:Agent
                                  ] ;
                  rdfs:comment "A relation between two Agents for the execution of an Activity. The relation involves one or more Rights of the agent which establishes the relation to the other agent." ;
                  rdfs:label "AgentRelation" .


###  http://w3id.org/semioe#Collaboration
ioe:Collaboration rdf:type owl:Class ;
                  rdfs:subClassOf ioe:AgentRelation ;
                  rdfs:comment "A type of ActorRelation which involves a collaboration between two Agents." ;
                  rdfs:label "Collaboration" .


###  http://w3id.org/semioe#CurrentRole
ioe:CurrentRole rdf:type owl:Class ;
                rdfs:subClassOf org:Role ;
                rdfs:comment "The current role of a foaf:Agent." ;
                rdfs:label "CurrentRole" .


###  http://w3id.org/semioe#Delegation
ioe:Delegation rdf:type owl:Class ;
               rdfs:subClassOf ioe:AgentRelation ;
               rdfs:comment "A type of ActorRelation which involves a delegation of tasks from an Agent to another Agent." ;
               rdfs:label "Delegation" .


###  http://w3id.org/semioe#HAgent
ioe:HAgent rdf:type owl:Class ;
           rdfs:subClassOf ioe:Agent ,
                           foaf:Agent ;
           rdfs:comment "A human agent." ;
           rdfs:label "HAgent" .



###  http://w3id.org/semioe#Process
ioe:Process rdf:type owl:Class ;
            rdfs:subClassOf ioe:WorkflowElement ;
            rdfs:comment "A process defined by the organization." ;
            rdfs:label "Process" .


###  http://w3id.org/semioe#Right
ioe:Right rdf:type owl:Class ;
          rdfs:subClassOf [ rdf:type owl:Restriction ;
                            owl:onProperty ioe:hasType ;
                            owl:someValuesFrom ioe:RightType
                          ] ;
          rdfs:comment "A right that can be associated to the ioe:CurrentRole of a foaf:Agent." ;
          rdfs:label "Right" .


###  http://w3id.org/semioe#RightOnEnvironment
ioe:RightOnEnvironment rdf:type owl:Class ;
                       rdfs:subClassOf ioe:Right ,
                                       [ rdf:type owl:Restriction ;
                                         owl:onProperty ioe:onEnvironment ;
                                         owl:someValuesFrom ioe:Site
                                       ] ;
                       rdfs:comment "A type of ioe:Right that is defined on all ioe:SmartObjects located in a ioe:Environment." ;
                       rdfs:label "RightOnEnvironment" .


###  http://w3id.org/semioe#RightOnSmartObject
ioe:RightOnSmartObject rdf:type owl:Class ;
                       rdfs:subClassOf ioe:Right ,
                                       [ rdf:type owl:Restriction ;
                                         owl:onProperty ioe:onSmartObject ;
                                         owl:someValuesFrom ioe:SmartObject
                                       ] ;
                       rdfs:comment "A type of ioe:Right that is defined on a ioe:SmartObject, including all its ssn:Systems." ;
                       rdfs:label "RightOnSmartObject" .


###  http://w3id.org/semioe#RightOnSystem
ioe:RightOnSystem rdf:type owl:Class ;
                  rdfs:subClassOf ioe:Right ,
                                  [ rdf:type owl:Restriction ;
                                    owl:onProperty ioe:onSystem ;
                                    owl:someValuesFrom ssn:System
                                  ] ;
                  rdfs:comment "A type of ioe:Right that is defined on a ioe:System." ;
                  rdfs:label "RightOnSystem" .


###  http://w3id.org/semioe#RightType
ioe:RightType rdf:type owl:Class ;
              rdfs:comment "The type of a ioe:Right, e.g. read, write." ;
              rdfs:label "RightType" .


###  http://w3id.org/semioe#Site
ioe:Site rdf:type owl:Class ;
         rdfs:subClassOf org:Site ,
                         bot:Site ;
         rdfs:comment "A location in the organization, e.g. a room, a building." ;
         rdfs:label "Site" .


###  http://w3id.org/semioe#SmartObject
ioe:SmartObject rdf:type owl:Class ;
                rdfs:subClassOf ioe:Agent ;
                rdfs:comment "A smart object in the IoE network, which can include one or more ssn:System." ;
                rdfs:label "SmartObject" .


###  http://w3id.org/semioe#System
ioe:System rdf:type owl:Class ;
           owl:equivalentClass [ rdf:type owl:Restriction ;
                                 owl:onProperty ioe:locatedIn ;
                                 owl:qualifiedCardinality "1"^^xsd:nonNegativeInteger ;
                                 owl:onClass ioe:SmartObject
                               ] ;
           rdfs:subClassOf ssn:System ;
           rdfs:comment "A system inside a SmartObject" ;
           rdfs:label "System" .


###  http://w3id.org/semioe#WorkflowElement
ioe:WorkflowElement rdf:type owl:Class ;
                    rdfs:comment "A generic workflow element, which can be either an ioe:Activity or an ioe:Process in the organization." ;
                    rdfs:label "WorkflowElement" .

